

# Complete Proof Generation Output

## User Request
Complete the following Lean 4 code:

```lean4
import Mathlib
import Aesop

set_option maxHeartbeats 0

open BigOperators Real Nat Topology Rat

theorem square_equation_solution {x y : ℝ} (h : x^2 + y^2 = 2*x - 4*y - 5) : x + y = -1 := by
  sorry
```

Before producing the Lean 4 code to formally prove the given theorem, provide a detailed proof plan outlining the main proof steps and strategies.
The plan should highlight key ideas, intermediate lemmas, and proof structures that will guide the construction of the final formal proof.

## Assistant Response

### Detailed Proof

**Problem:** Given real numbers \( x, y \) such that \( x^2 + y^2 = 2x - 4y - 5 \), prove that \( x + y = -1 \).

**Approach:**
1. Rearrange the equation to group all terms on one side to form a quadratic in terms of \( x \) or \( y \).
2. Complete the square for the quadratic terms to simplify the equation.
3. Use the simplified form to deduce a relationship between \( x \) and \( y \).
4. Derive the desired conclusion \( x + y = -1 \).

**Detailed Solution:**

1. Start with the given equation:
   \[ x^2 + y^2 = 2x - 4y - 5 \]

2. Move all terms to one side to set the equation to zero:
   \[ x^2 + y^2 - 2x + 4y + 5 = 0 \]

3. Complete the square for the \( x \)-terms and \( y \)-terms:
   - For \( x \): \( x^2 - 2x = (x - 1)^2 - 1 \)
   - For \( y \): \( y^2 + 4y = (y + 2)^2 - 4 \)

4. Substitute these back into the equation:
   \[ (x - 1)^2 - 1 + (y + 2)^2 - 4 + 5 = 0 \]
   Simplify the constants:
   \[ (x - 1)^2 + (y + 2)^2 - 1 - 4 + 5 = 0 \]
   \[ (x - 1)^2 + (y + 2)^2 = 0 \]

5. The sum of squares is zero if and only if each square is zero:
   \[ (x - 1)^2 = 0 \quad \text{and} \quad (y + 2)^2 = 0 \]
   This implies:
   \[ x - 1 = 0 \quad \text{and} \quad y + 2 = 0 \]
   \[ x = 1 \quad \text{and} \quad y = -2 \]

6. Compute \( x + y \):
   \[ x + y = 1 + (-2) = -1 \]

**Verification:**
Substitute \( x = 1 \) and \( y = -2 \) back into the original equation:
\[ 1^2 + (-2)^2 = 1 + 4 = 5 \]
\[ 2(1) - 4(-2) - 5 = 2 + 8 - 5 = 5 \]
Both sides are equal, so the solution is correct.

### Step 1: Abstract Plan

1. **Rearrange the Equation:**
   - Move all terms to one side to form a quadratic equation in \( x \) and \( y \).

2. **Complete the Square:**
   - For \( x \), complete the square to get \( (x - 1)^2 \).
   - For \( y \), complete the square to get \( (y + 2)^2 \).

3. **Simplify the Equation:**
   - Combine the completed squares to form a single equation of the form \( (x - 1)^2 + (y + 2)^2 = 0 \).

4. **Solve for \( x \) and \( y \):**
   - Since squares are non-negative and sum to zero, each square must be zero.
   - Deduce \( x = 1 \) and \( y = -2 \).

5. **Find \( x + y \):**
   - Compute \( x + y = -1 \).

### Step 2: Lean 4 `have` Statements

```lean4
theorem square_equation_solution {x y : ℝ} (h : x^2 + y^2 = 2*x - 4*y - 5) : x + y = -1 := by
  have h_main : (x - 1)^2 + (y + 2)^2 = 0 := by sorry
  have h_final : x + y = -1 := by sorry
  exact h_final
```

### Explanation:
1. `h_main`: This corresponds to the simplified equation after completing the square. The sum of squares is zero, which is derived from the given equation.
2. `h_final`: This is the conclusion \( x + y = -1 \), derived from the fact that the sum of squares is zero implies each square is zero, leading to \( x = 1 \) and \( y = -2 \).

### Complete Lean 4 Proof

```lean4
theorem square_equation_solution {x y : ℝ} (h : x^2 + y^2 = 2*x - 4*y - 5) : x + y = -1 := by
  have h_main : (x - 1)^2 + (y + 2)^2 = 0 := by
    have h1 : x^2 + y^2 = 2*x - 4*y - 5 := h
    have h2 : (x - 1)^2 + (y + 2)^2 = 0 := by
      nlinarith [sq_nonneg (x - 1 + (y + 2)), sq_nonneg (x - 1 - (y + 2)), sq_nonneg (x - 1 + (y + 2) - 2),
        sq_nonneg (x - 1 + (y + 2) + 2), sq_nonneg (x - 1 - (y + 2) - 2), sq_nonneg (x - 1 - (y + 2) + 2)]
    exact h2
  
  have h_final : x + y = -1 := by
    have h3 : (x - 1) ^ 2 + (y + 2) ^ 2 = 0 := h_main
    have h4 : (x - 1) ^ 2 = 0 := by
      nlinarith [sq_nonneg (y + 2), sq_nonneg (x - 1)]
    have h5 : (y + 2) ^ 2 = 0 := by
      nlinarith [sq_nonneg (y + 2), sq_nonneg (x - 1)]
    have h6 : x - 1 = 0 := by
      nlinarith
    have h7 : y + 2 = 0 := by
      nlinarith
    have h8 : x = 1 := by linarith
    have h9 : y = -2 := by linarith
    have h10 : x + y = -1 := by
      rw [h8, h9]
      norm_num
    exact h10
  
  exact h_final
```
